Pulled out correctness, started more efficient compiler

Compiler.thy
@@ -9,120 +9,49 @@ abbreviation code_compile :: "texpr \<Rightarrow> mach list" where
 abbreviation compile :: "nexpr \<rightharpoonup> mach list" where 
   "compile \<equiv> map_option (code_compile \<circ> fst) \<circ> typecheck"
 
-lemma [simp]: "live_frame (env, tco_cd (encode e), tco_r (encode e))"
-  by (induction e) simp_all
+primrec tree_code_size :: "tree_code \<Rightarrow> nat"
+    and tree_code_size_list :: "tree_code list \<Rightarrow> nat" where
+  "tree_code_size (TLookup x) = 0"
+| "tree_code_size (TPushCon k) = 0"
+| "tree_code_size (TPushLam cd) = tree_code_size_list cd"
+| "tree_code_size TApply = 0"
+| "tree_code_size_list [] = 1"
+| "tree_code_size_list (op # cd) = 
+      Suc (if op = TApply \<and> cd = [] then 0 else tree_code_size op + tree_code_size_list cd)"
 
-theorem tc_failure: "compile e = None \<Longrightarrow> \<nexists>e\<^sub>t t. (Map.empty \<turnstile>\<^sub>n e\<^sub>t : t) \<and> e = erase e\<^sub>t"
-proof -
-  assume "compile e = None"
-  hence "typecheck e = None" by simp
-  thus ?thesis by (metis typecheck_fails)
-qed
+primrec alg_compile1 :: "var list \<Rightarrow> texpr \<Rightarrow> tree_code list \<Rightarrow> tree_code list" where
+  "alg_compile1 \<Phi> (texpr.TVar x) acc = TLookup (the (idx_of \<Phi> x)) # acc"
+| "alg_compile1 \<Phi> (texpr.TConst k) acc = TPushCon k # acc"
+| "alg_compile1 \<Phi> (texpr.TLam x t e) acc = TPushLam (alg_compile1 (insert_at 0 x \<Phi>) e []) # acc"
+| "alg_compile1 \<Phi> (texpr.TApp e\<^sub>1 e\<^sub>2) acc = alg_compile1 \<Phi> e\<^sub>1 (alg_compile1 \<Phi> e\<^sub>2 (TApply # acc))"
 
-theorem tc_terminationn: "compile e = Some cd \<Longrightarrow> 
-  \<exists>v. valn v \<and> e \<Down> v \<and> (\<exists>rs mem. rs R3 = 1 \<and> rs R4 = 0 \<and> 
-    print_mval mem (4 * mem 2) = print_nexpr v \<and> 
-      iter (\<tturnstile> cd \<leadsto>\<^sub>m) (MS ((\<lambda>r. 0)(R4 := 1)) (nmem(3 := 0)) (length cd)) (MS rs mem 0))"
-proof -
-  assume C: "compile e = Some cd"
-  then obtain e\<^sub>t t where T: "typecheck e = Some (e\<^sub>t, t)" by fastforce
-  hence TN: "(Map.empty \<turnstile>\<^sub>n e\<^sub>t : t) \<and> e = erase e\<^sub>t" by simp
-  then obtain v\<^sub>t where ET: "e\<^sub>t \<Down>\<^sub>t v\<^sub>t" by fastforce
-  hence VT: "valt v\<^sub>t" by simp
-  hence VN: "valn (erase v\<^sub>t)" by simp
-  from ET have EN: "erase e\<^sub>t \<Down> erase v\<^sub>t" by simp
-  from TN have TD: "[] \<turnstile>\<^sub>d convert e\<^sub>t : t" by simp
-  from ET TN have ED: "convert e\<^sub>t \<Down>\<^sub>d convert v\<^sub>t" by fastforce
-  hence VD: "vald (convert v\<^sub>t)" by simp
-  from ED have "iter (\<leadsto>\<^sub>d) (convert e\<^sub>t) (convert v\<^sub>t)" by (metis BigStep.correctb)
-  with ED EN TD have ES: "iter (\<leadsto>\<^sub>s) (SS False [FReturn] (convert e\<^sub>t)) (SS True [] (convert v\<^sub>t))" 
-    by simp
-  from TD have TC: "CSE [CReturn []] [] (convert e\<^sub>t) :\<^sub>c t" 
-    by (metis tcc_state_ev tcc_nil tcc_snil tcc_scons_ret latest_environment.simps(4))
-  with ES VD EN obtain c where EC: "iter (\<leadsto>\<^sub>c) (CSE [CReturn []] [] (convert e\<^sub>t)) (CSC [] c) \<and> 
-    declosure c = convert v\<^sub>t" by fastforce
-  from TC EC have "iter (\<leadsto>\<^sub>t) (encode_state (CSE [CReturn []] [] (convert e\<^sub>t))) 
-    (encode_state (CSC [] c))" by (metis iter_completet)
-  hence "iter (\<leadsto>\<^sub>t) (TS [] [([], encode (convert e\<^sub>t))]) (TS [encode_closure c] [])" 
-    by (simp add: encode_def)
-  hence "iter (\<leadsto>\<^sub>t\<^sub>c\<^sub>o) (tco_state (TS [] [([], encode (convert e\<^sub>t))])) 
-    (tco_state (TS [encode_closure c] []))" by (metis iter_tco_eval)
-  hence ET: "iter (\<leadsto>\<^sub>t\<^sub>c\<^sub>o) (TCOS [] [([], tco_cd (encode (convert e\<^sub>t)), tco_r (encode (convert e\<^sub>t)))]) 
-    (TCOS [tco_val (encode_closure c)] [])" by simp
-  let ?cd = "(flatten_code \<circ> tco \<circ> encode \<circ> convert) e\<^sub>t"
-  have UB: "unflatten_state ?cd (BS [] [([], length ?cd)]) = 
-    TCOS [] [([], tco_cd (encode (convert e\<^sub>t)), tco_r (encode (convert e\<^sub>t)))]" 
-      by (auto simp add: tco_def simp del: flatten_code.simps)
-  have "orderly_state ?cd (BS [] [([], length ?cd)])" by auto
-  with ET UB obtain v\<^sub>b where EB: "iter (\<tturnstile> ?cd \<leadsto>\<^sub>b) (BS [] [([], length ?cd)]) (BS [v\<^sub>b] []) \<and> 
-    tco_val (encode_closure c) = unflatten_closure ?cd v\<^sub>b" by (metis evalb_end)
-  then obtain \<Sigma>\<^sub>h' where EH: "iter (\<tturnstile> ?cd \<leadsto>\<^sub>h) (HS hempty [] [([], length ?cd)]) \<Sigma>\<^sub>h' \<and> 
-    BS [v\<^sub>b] [] = unheap \<Sigma>\<^sub>h'" by fastforce
-  then obtain h\<^sub>h v\<^sub>h where SH: "\<Sigma>\<^sub>h' = HS h\<^sub>h [v\<^sub>h] [] \<and> v\<^sub>b = unheap_closure h\<^sub>h v\<^sub>h" 
-    using unheap_empty by blast
-  have HS: "heap_structured (HS hempty [] [([], length ?cd)])" by simp
-  have CES: "unchain_state (CES hempty hempty [] [(0, length ?cd)]) = 
-    HS hempty [] [([], length ?cd)]" by (simp add: unchain_stack_def)
-  with EH SH obtain \<Sigma>\<^sub>c\<^sub>e' where ECE: "iter (\<tturnstile> ?cd \<leadsto>\<^sub>c\<^sub>e) 
-    (CES hempty hempty [] [(0, length ?cd)]) \<Sigma>\<^sub>c\<^sub>e' \<and> HS h\<^sub>h [v\<^sub>h] [] = unchain_state \<Sigma>\<^sub>c\<^sub>e'" by fastforce
-  then obtain h\<^sub>c\<^sub>e env\<^sub>h where VCE: "\<Sigma>\<^sub>c\<^sub>e' = CES h\<^sub>c\<^sub>e env\<^sub>h [v\<^sub>h] [] \<and> h\<^sub>h = unchain_heap h\<^sub>c\<^sub>e env\<^sub>h" 
-    by (metis unchain_state_reverse map_is_Nil_conv unchain_stack_def)
-  have CS: "chained_state (CES hempty hempty [] [(0, length ?cd)])" by simp
-  with ECE VCE have "iter (\<tturnstile> ?cd \<leadsto>\<^sub>f) (flatten (CES hempty hempty [] [(0, length ?cd)]))
-    (flatten (CES h\<^sub>c\<^sub>e env\<^sub>h [v\<^sub>h] []))" by (metis completef_iter)
-  hence EF: "iter (\<tturnstile> ?cd \<leadsto>\<^sub>f) (FS (H nmem 0) (H nmem 0) [] [length ?cd, 0])
-     (FS (flatten_values h\<^sub>c\<^sub>e) (flatten_environment env\<^sub>h) [3 * v\<^sub>h] [])" by (simp add: hempty_def)
-  with ECE CS have "chained_state \<Sigma>\<^sub>c\<^sub>e'" by (metis preserve_chained)
-  with VCE have VH: "hcontains h\<^sub>c\<^sub>e v\<^sub>h" by simp
-  have "restructurable (US nmem 0 nmem 0 nmem 0 (nmem(0 := 0)) 1 (length ?cd)) ?cd" by simp
-  with EF have "\<exists>\<Sigma>\<^sub>u'. iter (\<tturnstile> ?cd \<leadsto>\<^sub>u) (US nmem 0 nmem 0 nmem 0 (nmem(0 := 0)) 1 (length ?cd)) \<Sigma>\<^sub>u' \<and>
-    FS (flatten_values h\<^sub>c\<^sub>e) (flatten_environment env\<^sub>h) [3 * v\<^sub>h] [] = restructure \<Sigma>\<^sub>u'" by simp_all
-  then obtain \<Sigma>\<^sub>u' where 
-    "iter (\<tturnstile> ?cd \<leadsto>\<^sub>u) (US nmem 0 nmem 0 nmem 0 (nmem(0 := 0)) 1 (length ?cd)) \<Sigma>\<^sub>u' \<and> 
-      FS (flatten_values h\<^sub>c\<^sub>e) (flatten_environment env\<^sub>h) [3 * v\<^sub>h] [] = restructure \<Sigma>\<^sub>u'" by blast
-  moreover then obtain h\<^sub>u hp\<^sub>u e\<^sub>u ep\<^sub>u vs\<^sub>u vp\<^sub>u sh\<^sub>u where VU:
-    "\<Sigma>\<^sub>u' = US h\<^sub>u hp\<^sub>u e\<^sub>u ep\<^sub>u vs\<^sub>u vp\<^sub>u sh\<^sub>u 0 0 \<and> flatten_values h\<^sub>c\<^sub>e = H h\<^sub>u hp\<^sub>u \<and> 
-      flatten_environment env\<^sub>h = H e\<^sub>u ep\<^sub>u \<and> listify' vs\<^sub>u vp\<^sub>u = 3 * v\<^sub>h # []" by auto
-  moreover hence VSU: "vs\<^sub>u 0 = 3 * v\<^sub>h \<and> vp\<^sub>u = 1" by auto
-  ultimately have "iter (\<tturnstile> ?cd \<leadsto>\<^sub>u) (US nmem 0 nmem 0 nmem 0 (nmem(0 := 0)) 1 (length ?cd)) 
-    (US h\<^sub>u hp\<^sub>u e\<^sub>u ep\<^sub>u vs\<^sub>u 1 sh\<^sub>u 0 0)" by simp
-  hence EU: "iter (\<tturnstile> ?cd \<leadsto>\<^sub>u) (US nmem 0 nmem 0 nmem 0 (nmem(0 := 0)) 1 (length ?cd)) 
-    (US h\<^sub>u hp\<^sub>u e\<^sub>u ep\<^sub>u vs\<^sub>u 1 sh\<^sub>u 0 0)" by simp
-  let ?mem = "(\<lambda>m. case m of Hp \<Rightarrow> h\<^sub>u | Env \<Rightarrow> e\<^sub>u | Val \<Rightarrow> vs\<^sub>u | Stk \<Rightarrow> sh\<^sub>u)"
-  let ?rs = "(\<lambda>r. case r of HP \<Rightarrow> hp\<^sub>u | EP \<Rightarrow> ep\<^sub>u | VP \<Rightarrow> Suc 0 | SP \<Rightarrow> 0 | ACC \<Rightarrow> 0 | AC2 \<Rightarrow> 0)"
-  let ?cd' = "(fst \<circ> assemble) ?cd"
+function alg_compile2 :: "nat \<Rightarrow> tree_code list \<Rightarrow> byte_code list \<Rightarrow> byte_code list" where
+  "alg_compile2 lib [] acc = BReturn # acc"
+| "alg_compile2 lib (TLookup x # cd) acc = alg_compile2 lib cd (BLookup x # acc)"
+| "alg_compile2 lib (TPushCon k # cd) acc = alg_compile2 lib cd (BPushCon k # acc)"
+| "alg_compile2 lib (TPushLam cd' # cd) acc =
+    alg_compile2 lib cd' 
+      (alg_compile2 (lib + tree_code_size_list cd') cd 
+        (BPushLam (lib + tree_code_size_list cd') # acc))"
+| "alg_compile2 lib (TApply # []) acc = BJump # acc"
+| "alg_compile2 lib (TApply # op # cd) acc = alg_compile2 lib (op # cd) (BApply # acc)"
+  by pat_completeness auto
+termination
+  by (relation "measure (tree_code_size_list \<circ> fst \<circ> snd)") simp_all
 
+definition alg_compile :: "texpr \<Rightarrow> byte_code list" where
+  "alg_compile e = alg_compile2 0 (alg_compile1 [] e []) []"
 
+lemma [simp]: "alg_compile1 \<Phi> e acc = encode (convert' \<Phi> e) @ acc"
+  by (induction e arbitrary: \<Phi> acc) simp_all
 
+lemma [simp]: "tree_code_size_list cd = code_list_size (tco_cd cd)"
+  by (induction cd rule: tco_cd.induct) (simp_all split: list.splits)
 
-  from C T obtain mp where MP: "assemble ?cd = (?cd', mp)" by (cases "assemble ?cd") simp_all
-  with EU have "iter (\<tturnstile> ?cd' \<leadsto>\<^sub>a) 
-    (assemble_state mp (US nmem 0 nmem 0 nmem 0 (nmem(0 := 0)) 1 (length ?cd))) 
-      (assemble_state mp (US h\<^sub>u hp\<^sub>u e\<^sub>u ep\<^sub>u vs\<^sub>u 1 sh\<^sub>u 0 0))" by (metis correcta_iter)
-  with MP have "iter (\<tturnstile> ?cd' \<leadsto>\<^sub>a) 
-    (AS (\<lambda>r. if r = SP then Suc 0 else 0) (\<lambda>m. if m = Stk then nmem(0 := 0) else nmem) 
-      (length ?cd')) (AS ?rs ?mem 0)" by simp
-  hence "iter (\<tturnstile> disassemble ?cd' \<leadsto>\<^sub>m) 
-    (disassemble_state (AS (\<lambda>r. if r = SP then Suc 0 else 0) 
-      (\<lambda>m. if m = Stk then nmem(0 := 0) else nmem) (length ?cd'))) 
-        (disassemble_state (AS ?rs ?mem 0))" by (metis correctm_iter)
-  with C T have EM: "iter (\<tturnstile> cd \<leadsto>\<^sub>m) (MS ((\<lambda>r. 0)(R4 := 1)) (nmem(3 := 0)) (length cd)) 
-    (MS (?rs \<circ> inv_register_map) (uncurry ?mem \<circ> unmap_mem) 0)" by auto
-  from EC VT have "print_closure c = print_nexpr (erase v\<^sub>t)" by simp
-  moreover from EB have "print_bclosure v\<^sub>b = print_tco_closure (tco_val (encode_closure c))" by simp
-  ultimately have "print_bclosure v\<^sub>b = print_nexpr (erase v\<^sub>t)" by simp
-  with SH have "print_hclosure (hlookup h\<^sub>h v\<^sub>h) = print_nexpr (erase v\<^sub>t)" by simp
-  with VCE VH have "print_ceclosure (hlookup h\<^sub>c\<^sub>e v\<^sub>h) = print_nexpr (erase v\<^sub>t)" by (metis print_ce)
-  with VH have "print_ceclosure (get_closure (flatten_values h\<^sub>c\<^sub>e) (3 * v\<^sub>h)) = print_nexpr (erase v\<^sub>t)" 
-    by (simp del: get_closure.simps)
-  with VU VSU have "print_uval h\<^sub>u (vs\<^sub>u 0) = print_nexpr (erase v\<^sub>t)" by (metis print_u)
-  hence PU: "print_uval (?mem Hp) (?mem Val 0) = print_nexpr (erase v\<^sub>t)" by simp
-  have "unmap_mem (4 * ?mem Val 0) = (Hp, ?mem Val 0)" by simp
-  hence "unmap_mem (4 * (uncurry ?mem \<circ> unmap_mem) 2) = (Hp, ?mem Val 0)" by (simp add: numeral_def)
-  with PU have PM: "print_mval (uncurry ?mem \<circ> unmap_mem) (4 * (uncurry ?mem \<circ> unmap_mem) 2) = 
-    print_nexpr (erase v\<^sub>t)" by (metis print_m)
-  have "(?rs \<circ> inv_register_map) R3 = 1 \<and> (?rs \<circ> inv_register_map) R4 = 0" by simp
-  with VN TN EN EM PM show ?thesis by blast
-qed
+lemma [simp]: "alg_compile2 lib cd acc = flatten_code' lib (tco_cd cd) (tco_r cd) @ acc"
+  by (induction lib cd acc rule: alg_compile2.induct) simp_all
+
+lemma [simp]: "alg_compile = flatten_code \<circ> tco \<circ> encode \<circ> convert"
+  by rule (simp add: alg_compile_def convert_def tco_def)
 
 end
